\begin{equation}
\begin{split}
    \underset{q^{g}(t), d^{g}(t), \ i \in \{L, H\}}{\max} \hspace{0.2cm} \int_{0}^{\infty} e^{-rt} \left\{ p(t) \sum_{g} q^{g}(t) \ - \ C\left( \sum_{g} d^{g}(t) \right) \right\} dt
\end{split}
\label{Equation:AKS-Style-Model_Objective-Function}
\end{equation}
subject to
\begin{equation}
\begin{split}
    \dot{K}(t) \ = \ - \delta \sum_{g} q^{g}(t) \ + \ \sum_{g} I^{g} d^{g}(t), \hspace{0.3cm} K_{0} \ = \ K(0) \ \text{given,}
\end{split}
\end{equation}
\begin{equation}
\begin{split}
    \dot{R}^{g}(t) \ = \ - d^{g}(t), \hspace{0.3cm} R_{0}^{g} \ = \ R^{g}(0) \ \text{given,} 
\end{split}
\end{equation}
\begin{equation}
\begin{split}
    q^{g}(t) \ \geq \ 0, \hspace{0.3cm} 0 \ \leq \ \sum_{g} q^{g}(t) \ \leq \ K(t),
\end{split}
\end{equation}
\begin{equation}
\begin{split}
    d^{g}(t) \ \geq \ 0, \hspace{0.3cm} R^{g}(t) \ \geq \ 0.
\end{split}
\end{equation}
