\begin{equation}
\begin{split}
%    f_{ik} (p_{k}; \boldsymbol{\theta_{f}})
%    f_{ik} (\boldsymbol{x}_{ik}; \boldsymbol{\theta}_{f}) \
%    & = \ 
%    \begin{cases}
%        \ \widetilde{f}_{ik} (g_{ik}, p_{k}; \boldsymbol{\theta}_{f}) \hspace{0.5cm} \text{if $s_{ik} = 0$} \\
%        \ 0  \hspace{2.55cm} \text{if $s_{ik} = 1$}.
%    \end{cases}
%    & = \ (1 - s_{ik}) \big\{ \theta_{1} \ + \ \theta_{2}p_{k} \ + \ \theta_{3}(1 - g_{ik}^{L}) \big\}.
\end{split}
\label{Equation:Firms-Problem_Flow-Payoff}
\end{equation}